Trestle/Encode/Tseitin.lean
@@ -101,24 +101,46 @@ theorem toPropFun_ofPropForm (f : PropForm ν)
 mutual
 def conjuncts : NegNormForm ν → Array (NegNormForm ν)
 | lit l => #[.lit l]
-| all as => as.attach.flatMap (fun ⟨a,_h⟩ => conjuncts a)
+| all as => as.attach.flatMap (fun ⟨a,h⟩ => conjuncts a)
 | any as =>
-  let disj := as.attach.flatMap (fun ⟨a,_h⟩ => disjuncts a)
+  let disj := as.attach.flatMap (fun ⟨a,h⟩ => disjuncts a)
   if h : disj.size = 1 then
     #[disj[0]]
   else
     #[.any disj]
+termination_by f => sizeOf f
+decreasing_by
+  all_goals (
+    simp_wf
+    first
+    | have := Array.sizeOf_lt_of_mem h
+      omega
+    | rename_i hx
+      have := Array.sizeOf_lt_of_mem hx.property
+      omega
+  )
 
 def disjuncts : NegNormForm ν → Array (NegNormForm ν)
 | lit l => #[.lit l]
-| any as => as.attach.flatMap (fun ⟨a,_h⟩ => disjuncts a)
+| any as => as.attach.flatMap (fun ⟨a,h⟩ => disjuncts a)
 | all as =>
-  let conj := as.attach.flatMap (fun ⟨a,_h⟩ => conjuncts a)
+  let conj := as.attach.flatMap (fun ⟨a,h⟩ => conjuncts a)
   if h : conj.size = 1 then
     #[conj[0]]
   else
-    #[.all <| conj]
-end
+    #[.all conj]
+termination_by f => sizeOf f
+decreasing_by
+  all_goals (
+    simp_wf
+    first
+    | have := Array.sizeOf_lt_of_mem h
+      omega
+    | rename_i hx
+      have := Array.sizeOf_lt_of_mem hx.property
+      omega
+  )
+end /- mutual -/
 
 set_option maxHeartbeats 500000 in
 set_option pp.proofs.withType false in
@@ -127,7 +149,7 @@ def toPropFun_all_conjuncts : (f : NegNormForm ν) → toPropFun (.all (conjunct
 | lit l => by simp [conjuncts, toPropFun, Array.attach, PropFun.all]
 | all as => by
   have IH : ∀ a ∈ as, _ := fun a _h => toPropFun_all_conjuncts a
-  rcases as with ⟨as⟩; simp only [Array.mem_toArray] at IH
+  rcases as with ⟨as⟩; simp only [List.mem_toArray] at IH
   ext τ
   replace IH := open PropFun in fun a ha => congrArg (τ ⊨ ·) (IH a ha).symm
   simp [conjuncts, toPropFun, List.unattach, -List.map_subtype] at IH ⊢
@@ -137,10 +159,10 @@ def toPropFun_all_conjuncts : (f : NegNormForm ν) → toPropFun (.all (conjunct
   lift_lets; intro disj
   have : toPropFun (any disj) = toPropFun (any as) := by
     have IH : ∀ a ∈ as, _ := fun a _h => toPropFun_any_disjuncts a
-    rcases as with ⟨as⟩; simp only [Array.mem_toArray] at IH
+    rcases as with ⟨as⟩; simp only [List.mem_toArray] at IH
     ext τ
     replace IH := open PropFun in fun a ha => congrArg (τ ⊨ ·) (IH a ha).symm
-    simp [disj, disjuncts, toPropFun, List.unattach, -List.map_subtype] at IH ⊢
+    simp [disj, toPropFun, List.unattach, -List.map_subtype] at IH ⊢
     aesop
   rw [← this]; clear this
   ext τ
@@ -155,7 +177,7 @@ def toPropFun_any_disjuncts : (f : NegNormForm ν) → toPropFun (.any (disjunct
 | lit l => by simp [disjuncts, toPropFun, Array.attach, PropFun.any]
 | any as => by
   have IH : ∀ a ∈ as, _ := fun a _h => toPropFun_any_disjuncts a
-  rcases as with ⟨as⟩; simp only [Array.mem_toArray] at IH
+  rcases as with ⟨as⟩; simp only [List.mem_toArray] at IH
   ext τ
   replace IH := open PropFun in fun a ha => congrArg (τ ⊨ ·) (IH a ha).symm
   simp [disjuncts, toPropFun, List.unattach, -List.map_subtype] at IH ⊢
@@ -165,10 +187,10 @@ def toPropFun_any_disjuncts : (f : NegNormForm ν) → toPropFun (.any (disjunct
   lift_lets; intro conj
   have : toPropFun (all conj) = toPropFun (all as) := by
     have IH : ∀ a ∈ as, _ := fun a _h => toPropFun_all_conjuncts a
-    rcases as with ⟨as⟩; simp only [Array.mem_toArray] at IH
+    rcases as with ⟨as⟩; simp only [List.mem_toArray] at IH
     ext τ
     replace IH := open PropFun in fun a ha => congrArg (τ ⊨ ·) (IH a ha).symm
-    simp [conj, conjuncts, toPropFun, List.unattach, -List.map_subtype] at IH ⊢
+    simp [conj, toPropFun, List.unattach, -List.map_subtype] at IH ⊢
     aesop
   rw [← this]; clear this
   ext τ
@@ -351,7 +373,7 @@ def encodeNNF
             rcases this with ⟨i,hi,this⟩
             use Literal.pos (Sum.inr ⟨i,hi⟩)
             constructor
-            · right; simp [Array.mem_def, List.mem_ofFn]
+            · right; simp
             · simp +zetaDelta [this, h]
       )
 termination_by sizeOf f
